.. _palindromics-introduction:

Introduction
============

.. toctree::
   :maxdepth: 1
   :caption: Contents:
   :hidden:

   intro-i_overview
   intro-ii_motivation

.. _palindromics-table-of-contents:

Table Of Contents
-----------------

- :ref:`Introduction <palindromics-introduction>`
    - :ref:`Table of Content <palindromics-table-of-contents>`
    - :ref:`Glossary <palindromics-glossary>`
    - :ref:`Overview <palindromics-overview>`
    - :ref:`Motivation <palindromics-motivation>`
- :ref:`Section I: Languages & Corpora <palindromics-section-i>`
    - :ref:`I.I: Formalization <palindromics-section-i-i>`
    - :ref:`I.II: Strings <palindromics-section-i-ii>`
    - :ref:`I.III: Words <palindromics-section-i-iii>`
    - :ref:`I.IV: Sentences <palindromics-section-i-iv>`
    - :ref:`I.V: Summary <palindromics-section-i-v>`
- :ref:`Section II: Structures <palindromics-section-ii>`
    - :ref:`II.I: Delimiter Count <palindromics-section-ii-i>`
    - :ref:`II.II: Pivots <palindromics-section-ii-ii>`
    - :ref:`II.III: Reductions <palindromics-section-ii-iii>`
    - :ref:`II.IV: Palindromes <palindromics-section-ii-iv>`
    - :ref:`II.V: Summary <palindromics-section-ii-v>`
- :ref:`Section III: Postulates <palindromics-section-iii>`
    - :ref:`III.I: Prior Results <palindromics-section-iii-i>`
    - :ref:`III.II: Inverse Postulates <palindromics-section-iii-ii>`
    - :ref:`III.III: Summary <palindromics-section-iii-iii>`
- :ref:`Section IV: Analysis <palindromics-section-iv>`
    - :ref:`IV.I: Sentence Integrals <palindromics-section-iv-i>`
    - :ref:`IV.II: Probability <palindromics-section-iv-ii>`
    - :ref:`IV.III: Summary <palindromics-section-iv-iii>`
- :ref:`Appendix I: Addendums <palindromics-appendix-i>`
    - :ref:`AI.I: Omitted Axioms <palindromics-appendix-i-i>`
    - :ref:`AI.II: Omitted Proofs <palindromics-appendix-i-ii>`
- :ref:`Appendix II: Data <palindromics-appendix-ii>`
    - :ref:`AII.I: English Data <palindromics-appendix-ii-i>`
    - :ref:`AII.II: Latin Data <palindromics-appendix-ii-ii>`
- :ref:`Appendix III: Code <palindromics-appendix-iii>`

.. _palindromics-glossary:

Glossary
--------

.. NOTE: Glossary isn't done yet.

.. _palindromics-definitions:

-----------
Definitions
-----------

1. :ref:`Definition 1.2.1: Concatenation <palindromics-definition-1-2-1>`: :math:`st`
2. :ref:`Definition 1.2.2: String Length <palindromics-definition-1-2-2>`: :math:`l(s)`
3. :ref:`Definition 1.2.3: Character Indices <palindromics-definition-1-2-3>`: :math:`s[i]`
4. :ref:`Definition 1.2.5: Containment <palindromics-definition-1-2-5>`: :math:`t \subset_s s`
5. :ref:`Definition 1.2.6: Canonization <palindromics-definition-1-2-6>`: :math:`\pi(s)`
6. :ref:`Definition 1.2.7: Canon <palindromics-definition-1-2-7>`: :math:`\mathbb{S} = \{ \pi(s) \mid s \in S \}` 
7. :ref:`Definition 1.2.8: String Inversion <palindromics-definition-1-2-8>`: :math:`s^{-1}`
8. :ref:`Definition 1.3.1: Reflective Words <palindromics-definition-1-3-1>`: :math:`\alpha \in R \equiv \alpha = {\alpha}^{-1}`
9. :ref:`Definition 1.3.2: Invertible Words <palindromics-definition-1-3-2>` :math:`\alpha \in I \equiv {\alpha}^{-1} \in L`
10. :ref:`Definition 1.3.3: Phrases <palindromics-definition-1-3-3>`: :math:`P_n = (p(1), ..., p(n))`
11. :ref:`Definition 1.3.4: Lexicons <palindromics-definition-1-3-4>`: :math:`L_n = \{ p \mid \forall p: p = P_n \}`
12. :ref:`Definition 1.3.5: Limitation <palindromics-definition-1-3-5>`: :math:`\Pi_{i=1}^{n} p(i)`
13. :ref:`Definition 1.3.6: Dialect <palindromics-definition-1-3-6>`: :math:`D = \bigcup_{i=1}^{\infty} \{ s \in S \mid \exists p \in L_i: s = \Pi_{j=1}^{i} p(j) \}`
14. :ref:`Definition 1.4.1: Word Length <palindromics-definition-1-4-1>`: :math:`\Lambda(\zeta)`
15. :ref:`Definition 1.4.2: Word Indices <palindromics-definition-1-4-2>`: :math:`\zeta[[i]]`
16. :ref:`Definition 1.4.3: Invertible Sentences <palindromics-definition-1-4-3>`: :math:`\zeta \in J \equiv {\zeta}^{-1} \in C`
17. :ref:`Definition 1.4.4: Partial Sentences <palindromics-definition-1-4-4>`: :math:`\zeta[i:], \zeta[:i]`
18. :ref:`Definition 2.1.1: Delimiter Count <palindromics-definition-2-1-1>`: :math:`\Delta(s)`
19. :ref:`Definition 2.2.1: Pivot Characters <palindromics-definition-2-2-1>`: :math:`\overleftarrow{\omega_s}, \overrightarrow{\omega_s}, \omega_s`
20. :ref:`Definition 2.2.2: Pivot Words <palindromics-definition-2-2-2>`: :math:`\overleftarrow{\Omega_{\zeta}}, \overrightarrow{\Omega_{\zeta}}, \Omega_{\zeta}`
21. :ref:`Definition 2.2.3: Subvertible Sentences <palindromics-definition-2-2-3>`: :math:`\zeta \in \cancel{J} \equiv (\Omega_\zeta \neq \varepsilon) \land (\omega_\zeta \neq \varepsilon)`
22. :ref:`Definition 2.3.1: Ïƒ-Reduction <palindromics-definition-2-3-1>`: :math:`\varsigma(s)`
23. :ref:`Definition 2.4.1: Palindromes <palindromics-definition-2-4-1>`: :math:`\zeta \in P \equiv ((\varsigma(s)) = \varsigma(s)^{-1})`
24. :ref:`Definition 2.4.2: Perfect Palindromes <palindromics-definition-2-4-2>`: :math:`\zeta \in K \equiv (\zeta = \zeta^{-1})`
25. :ref:`Definition 2.4.3: Imperfect Palindromes <palindromics-definition-2-4-3>`: 

.. _palindromics-axioms:

------
Axioms
------

1. :ref:`Axiom 0: Empty Axiom <palindromics-axiom-0>`: :math:`\exists! \varepsilon`
2. :ref:`Axiom I: Comprehension Axiom <palindromics-axiom-i>`: :math:`\iota \in S`
3. :ref:`Axiom II: Equality Axiom <palindromics-axiom-ii>`: :math:`s = t`
4. :ref:`Axiom III: Closure Axiom <palindromics-axiom-iii>`: :math:`st \in S`
5. :ref:`Axiom IV: Measure Axiom <palindromics-axiom-iv>`: :math:`l(\alpha) \neq 0`
6. :ref:`Axiom V: Discovery Axiom <palindromics-axiom-v>`: :math:`\alpha[i] \neq \sigma`
7. :ref:`Axiom VI: Canonization Axiom <palindromics-axiom-vi>`: :math:`\alpha \in \mathbb{S}`

.. _palindromics-theorems:

--------
Theorems
--------

1. :ref:`Theorem 1.2.1 <palindromics-theorem-1-2-1>`: :math:`l(st) = l(s) + l(t)`
2. :ref:`Theorem 1.2.2 <palindromics-theorem-1-2-2>`: :math:`\varepsilon \subset_s s`
3. :ref:`Theorem 1.2.3 <palindromics-theorem-1-2-3>`: :math:`(\iota \subset_s uv) \implies ((\iota \subset_s u) \lor (\iota \subset_s v))`
4. :ref:`Theorem 1.2.4 <palindromics-theorem-1-2-4>`: :math:`\pi(\pi(s)) = \pi(s)`
5. :ref:`Theorem 1.2.5 <palindromics-theorem-1-2-5>`: :math:`s \in \mathbb{S} \equiv \pi(s) = s`
6. :ref:`Theorem 1.2.6 <palindromics-theorem-1-2-6>`: :math:`s,t \in \mathbb{S} \implies st \in \mathbb{S}`
7. :ref:`Theorem 1.2.8 <palindromics-theorem-1-2-8>`: :math:`\forall s \in \mathbb{S}: ((l(s) = l(t)) \land (\forall i \in N_{l(t)}: s[i] = t[i])) \implies (s = t)`
8. :ref:`Theorem 1.2.9 <palindromics-theorem-1-2-9>`: :math:`(s^{-1})^{-1} = s`
9. :ref:`Theorem 1.2.10 <palindromics-theorem-1-2-10>`: :math:`(st)^{-1} = (t^{-1})(s^{-1})`
10. :ref:`Theorem 1.2.11 <palindromics-theorem-1-2-11>`: :math:`u \subset_s v \equiv u^{-1} \subset_s v^{-1}`
11. :ref:`Theorem 1.3.1 <palindromics-theorem-1-3-1>`: :math:`\alpha \in I \equiv {\alpha}^{-1} \in I`
12. :ref:`Theorem 1.3.2 <palindromics-theorem-1-3-2>`: :math:`R \subset I`
13. :ref:`Theorem 1.3.3 <palindromics-theorem-1-3-3>`: :math:`\exists! s = \Pi_{i=1}^{n} p(i)` 
14. :ref:`Theorem 1.3.4 <palindromics-theorem-1-3-4>`: :math:`\forall s \in D: \nexists i: (s[i+1] = \sigma) \land (s[i] = \sigma)`
15. :ref:`Theorem 1.4.1 <palindromics-theorem-1-4-1>`: :math:`\sum_{j=1}^{\Lambda(\zeta)} l(\zeta[[j]]) \geq \Lambda(\zeta)`
16. :ref:`Theorem 1.4.2 <palindromics-theorem-1-4-2>`: :math:`\Lambda(\zeta\xi) \leq \Lambda(\zeta) + \Lambda(\xi)` 
17. :ref:`Theorem 1.4.3 <palindromics-theorem-1-4-3>`: :math:`\zeta = \Pi_{i=1}^{\Lambda(\zeta)} \zeta[[i]]`
18. :ref:`Theorem 1.4.4 <palindromics-theorem-1-4-4>`: :math:`(\Pi_{i=1}^{\Lambda(\zeta)} \zeta[[i]])^{-1} = \Pi_{i=1}^{\Lambda(\zeta)} (\zeta[[\Lambda(\zeta) - i + 1]])^{-1}`
19. :ref:`Theorem 1.4.5 <palindromics-theorem-1-4-5>`: :math:`\Lambda((s)(\sigma)(t)) = \Lambda(s) + \Lambda(t)`
20. :ref:`Theorem 1.4.6 <palindromics-theorem-1-4-6>`: :math:`C \subseteq D`
21. :ref:`Theorem 1.4.7 <palindromics-theorem-1-4-7>`: :math:`\Lambda((\zeta)(\sigma)(\xi)) = \Lambda(\zeta) + \Lambda(\xi)`
22. :ref:`Theorem 1.4.8 <palindromics-theorem-1-4-8>`: :math:`C \subseteq \mathbb{S}`
23. :ref:`Theorem 1.4.9 <palindromics-theorem-1-4-9>`: :math:`\zeta \in J \equiv {\zeta}^{-1} \in J`
24. :ref:`Theorem 1.4.10 <palindromics-theorem-1-4-10>`: :math:`\zeta \in J \implies \zeta[[i]] \in I`
25. :ref:`Theorem 1.4.11 <palindromics-theorem-1-4-11>`: :math:`\zeta \in J \implies {\zeta}^{-1}[[i]] = (\zeta[[\Lambda(\zeta) - i + 1]])^{-1}`
26. :ref:`Theorem 1.4.12 <palindromics-theorem-1-4-12>`: :math:`\zeta \in J \implies (\Lambda(\zeta) = \Lamdab(\zeta^{-1}))`
27. :ref:`Theorem 1.4.13 <palindromics-theorem-1-4-13>`: :math:`l(s[:i]) = i`
28. :ref:`Theorem 1.4.14 <palindromics-theorem-1-4-14>`: :math:`l(s[i:]) = l(s) - i + 1`
29. :ref:`Theorem 1.4.15 <palindromics-theorem-1-4-15>`: :math:`s[:l(s)] = s`
30. :ref:`Theorem 1.4.16 <palindromics-theorem-1-4-16>`: :math:`s[1:] = s`
31. :ref:`Theorem 1.4.17 <palindromics-theorem-1-4-15>`: :math:`s = (s[:i])(s[i+1:])`
32. :ref:`Theorem 2.1.1 <palindromics-theorem-2-1-1>`: :math:`\Lambda(\zeta) = \Delta(\zeta) + 1`
33. :ref:`Theorem 2.1.2 <palindromics-theorem-2-1-1>`: :math:`\Delta(s) = \Delta(s^{-1})`
34. :ref:`Theorem 2.1.3 <palindromics-theorem-2-1-3>`: :math:`l(\zeta) = \Delta(\zeta) + \sum_{i=1}^{\Lambda(\zeta)} l(\zeta[[i]])`
35. :ref:`Theorem 2.1.4 <palindromics-theorem-2-1-4>`: :math:`\Delta(st) = \Delta(s) + \Delta(t)`
36. :ref:`Theorem 2.1.5 <palindromics-theorem-2-1-5>`: :math:`((\Delta(s) = 2n +1) \land (s = s^{-1})) \implies (s[\frac{l(s)+1}{2}] = \sigma)`
37. :ref:`Theorem 2.1.6 <palindromics-theorem-2-1-6>`: :math:`((\Delta(s) = 2n + 1) \land (s = s^{-1})) \implies \exists i: l(s) = 2i - 1`
38. :ref:`Theorem 2.2.1 <palindromics-theorem-2-2-1>`: :math:`((\Delta(s) = 2n + 1) \land (s = s^{-1})) \implies (\overrightarrow{\omega_s} = \overleftarrow{\omega_s})`
39. :ref:`Theorem 2.2.2 <palindromics-theorem-2-2-2>`: :math:`((\Delta(s) = 2n) \land (s = s^{-1})) \implies ((\overrightarrow{\omega_s} \neq \sigma) \land (\overleftarrow{\omega_s} \neq \sigma))`
40. :ref:`Theorem 2.2.3 <palindromics-theorem-2-2-3>`: :math:`((\Delta(s) = 2n) \land (s = s^{-1})) \implies (\overrightarrow{\omega_s} = \overleftarrow{\omega_s})`
41. :ref:`Theorem 2.2.4 <palindromics-theorem-2-2-4>`: :math:`(s = s^{-1}) \implies (\omega_s \neq \varepsilon)`
42. :ref:`Theorem 2.2.5 <palindromics-theorem-2-2-5>`: :math:`((\Delta(\zeta) = 2i) \land (\Omega_{\zeta} \neq \varepsilon)) \implies (\Omega_{\zeta} \in R)`
43. :ref:`Theorem 2.2.6 <palindromics-theorem-2-2-6>`: :math:`((\Delta(\zeta) = 2i + 1) \land (\Omega_{\zeta} \neq \varepsilon)) \implies (\Omega_{\zeta} \in I)`
44. :ref:`Theorem 2.2.7 <palindromics-theorem-2-2-7>`: IN PROGRESS
45. :ref:`Theorem 2.2.8 <palindromics-theorem-2-2-8>`: IN PROGRESS
46. :ref:`Theorem 2.3.1 <palindromics-theorem-2-3-1>`: :math:`\varsigma(st) = (\varsigma(s))(\varsigma(t))`
47. :ref:`Theorem 2.3.2 <palindromics-theorem-2-3-2>`: :math:`\Delta(s) = 0 \equiv \varsigma(s) = s`
48. :ref:`Theorem 2.3.4 <palindromics-theorem-2-3-4>`: :math:`(\varsigma(s))^{-1} = \varsigma(s^{-1})`
49. :ref:`Theorem 2.3.5 <palindromics-theorem-2-3-5>`: :math:`\varsigma(\varsigma(s)) = \varsigma(s)`
50. :ref:`Theorem 2.3.6 <palindromics-theorem-2-3-6>`: :math:`s \subset_s t \equiv \varsigma(s) \subset_s \varsigma(t)`
51. :ref:`Theorem 2.3.7 <palindromics-theorem-2-3-7>`: :math:`\zeta[[i]] \subset_s \varsigma(\zeta)`
52. :ref:`Theorem 2.4.1 <palindromics-theorem-2-3-1>`: :math:`K \subseteq J`
53. :ref:`Theorem 2.4.2 <palindromics-theorem-2-4-2>`: :math:`\zeta \in K \implies \zeta[[i]] \in I`
54. :ref:`Theorem 2.4.3 <palindromics-theorem-2-4-3>`: :math:`\zeta \in K \implies \zeta^{-1}[[i]] = (\zeta[[\Lambda(\zeta) - 1 +1]])^{-1}`
55. :ref:`Theorem 2.4.4 <palindromics-theorem-2-4-4>`: :math:`\zeta \in K \imples \Lambda(zeta) = \Lambda(zeta^{-1})`
56. :ref:`Theorem 2.4.5 <palindromics-theorem-2-4-5>`: :math:`K \subseteq P`
57. :ref:`Theorem 2.4.6 <palindromics-theorem-2-4-6>`: :math:`\zeta \in K \implies (\omega_{\zeta} \neq \varepsilon)`
58. :ref:`Theorem 2.4.7 <palindromics-theorem-2-4-7>`: :math:`\zeta \in K \imples (\Omega_{\zeta} \neq \varepsilon)`
59. :ref:`Theorem 2.4.8 <palindromics-theorem-2-4-8>`: :math:`K \subseteq \cancel{J}`
60. :ref:`Theorem 3.2.1 <palindromics-theorem-3-2-1>`: :math:`\zeta \in K \implies ((\omega_{\zeta} = \sigma) \equiv (\zeta \in P_{-}))`
61. :ref:`Theorem 3.2.2 <palindromics-theorem-3-2-2>`: :math:`\zeta \in K \implies ((\omega_{\zeta} \neq \sigma) \equiv (\Omega_{\zeta} \in R))`
62. :ref:`Theorem 3.2.3 <palindromics-theorem-3-2-3>`: :math:`\zeta \in K \implies ((\omega_{\zeta} \neq \sigma) \equiv (\omega_{\Omega_{\zeta}} = \omega_{\zeta}))`
